case-studies/kathrin/coq-setoid-funcomp/Chapter9/preservation.v
@@ -28,7 +28,7 @@ Definition ltc {k k'} (Gamma: ctx k) (Delta: ctx k') rho := forall x, Delta (rho
 Lemma typing_ren n k (Gamma: ctx n) (Delta: ctx k) (rho: fin n -> fin k) (M: tm n) T :
   ltc Gamma Delta rho  -> Gamma |- M : T ->  Delta |- (M⟨rho⟩) : T.
 Proof.
-  intros C H. revert k Delta rho C. induction H; intros; cbn; eauto using has_type.
+  intros C H. revert k Delta rho C. induction H; intros; cbn; eauto.
   - unfold ltc in C. rewrite <- C. constructor.
   - constructor. apply IHhas_type. asimpl. unfold ltc. auto_case.
   - econstructor; eauto.
@@ -37,8 +37,7 @@ Qed.
 Lemma typing_inst n k (Gamma: ctx n) (Delta: ctx k) (sigma: fin n -> tm k) (M: tm n) T :
   (forall x, Delta |- sigma x : Gamma x) -> Gamma |- M : T ->  Delta |- (M[sigma]) : T.
 Proof.
-  intros C H. revert k Delta sigma C. induction H; intros; asimpl; eauto using has_type.
-  - apply C.
+  intros C H. revert k Delta sigma C. induction H; intros; asimpl; eauto.
   - constructor. apply IHhas_type. auto_case.
     + eapply typing_ren; eauto. intros. unfold ltc. now asimpl.
     + constructor.
